FMT/API.lean
@@ -1,14 +1,7 @@
 import FMT.Types.LocalType
-import FMT.Invariants.Eval
 
 namespace FMT.API
 
-def evalAPI (t : FMT.Types.LocalType) : Nat :=
-  match t with
-  | true => 1
-  | false => 0
-
-theorem evalAPI_spec (t : FMT.Types.LocalType) :
-  evalAPI t = (match t with | true => 1 | false => 0) := rfl
+def useLocalType : FMT.Types.LocalType := true
 
 end FMT.API
